src/program_proof/pav/rpc.v
@@ -5,33 +5,33 @@ From Perennial.program_proof.pav Require Import auditor advrpc core serde server
 
 Section specs.
 Context `{!heapGS Σ, !pavG Σ}.
-Lemma wp_newRpcServer ptr_serv serv :
+Lemma wp_NewRpcServer ptr_serv serv :
   {{{
     "Hown_serv" ∷ server.Server.own ptr_serv serv
   }}}
-  newRpcServer #ptr_serv
+  NewRpcServer #ptr_serv
   {{{
     ptr_rpcserv rpcserv, RET #ptr_rpcserv;
     "Hown_rpcserv" ∷ advrpc.Server.own ptr_rpcserv rpcserv
   }}}.
 Proof. Admitted.
 
-Lemma wp_newRpcAuditor ptr_adtr :
+Lemma wp_NewRpcAuditor ptr_adtr :
   {{{
     "Hown_adtr" ∷ Auditor.valid ptr_adtr
   }}}
-  newRpcAuditor #ptr_adtr
+  NewRpcAuditor #ptr_adtr
   {{{
     ptr_rpcserv rpcserv, RET #ptr_rpcserv;
     "Hown_rpcserv" ∷ advrpc.Server.own ptr_rpcserv rpcserv
   }}}.
 Proof. Admitted.
 
-Lemma wp_callServAudit ptr_cli cli (ep : w64) :
+Lemma wp_CallServAudit ptr_cli cli (ep : w64) :
   {{{
     "Hown_cli" ∷ advrpc.Client.own ptr_cli cli
   }}}
-  callServAudit #ptr_cli #ep
+  CallServAudit #ptr_cli #ep
   {{{
     ptr_upd upd (err : bool), RET (#ptr_upd, #err);
     "Hown_cli" ∷ advrpc.Client.own ptr_cli cli ∗
@@ -41,12 +41,12 @@ Lemma wp_callServAudit ptr_cli cli (ep : w64) :
   }}}.
 Proof. Admitted.
 
-Lemma wp_callAdtrUpdate ptr_cli cli ptr_upd upd :
+Lemma wp_CallAdtrUpdate ptr_cli cli ptr_upd upd :
   {{{
     "Hown_cli" ∷ advrpc.Client.own ptr_cli cli ∗
     "Hown_upd" ∷ UpdateProof.own ptr_upd upd
   }}}
-  callAdtrUpdate #ptr_cli #ptr_upd
+  CallAdtrUpdate #ptr_cli #ptr_upd
   {{{
     (err : bool), RET #err;
     "Hown_cli" ∷ advrpc.Client.own ptr_cli cli ∗
@@ -54,11 +54,11 @@ Lemma wp_callAdtrUpdate ptr_cli cli ptr_upd upd :
   }}}.
 Proof. Admitted.
 
-Lemma wp_callAdtrGet ptr_cli cli (ep : w64) :
+Lemma wp_CallAdtrGet ptr_cli cli (ep : w64) :
   {{{
     "Hown_cli" ∷ advrpc.Client.own ptr_cli cli
   }}}
-  callAdtrGet #ptr_cli #ep
+  CallAdtrGet #ptr_cli #ep
   {{{
     ptr_adtrInfo adtrInfo (err : bool), RET (#ptr_adtrInfo, #err);
     "Hown_cli" ∷ advrpc.Client.own ptr_cli cli ∗
